\documentclass[a4paper,12pt]{report}

\usepackage[margin=0.9in]{geometry}
\usepackage{graphicx}
\usepackage{float}
\usepackage[utf8]{inputenc}
\usepackage[T2A]{fontenc}
\usepackage{textcomp}
\usepackage{amsmath, amssymb}
\usepackage{siunitx}
\usepackage{mathtools}% http://ctan.org/pkg/mathtools
\usepackage{cancel}
\usepackage{xcolor}
\usepackage{bm}

\definecolor{grey}{HTML}{737373}

\begin{document}

\begin{enumerate}
  \item Ищем центр скоростей по формуле Эйлера.

\[
\vec{v}_B = \vec{v}_A + \vec{\omega} \times \vec{AB}
.\] 

\[
  \begin{pmatrix} 
    v_{Bx} - v_{Ax} \\
    v_{By} - v_{Ay} \\
    0
  \end{pmatrix} 
  \begin{pmatrix}
    -\omega \cdot \left( y_B - y_A \right) \\
    \omega \cdot ( x_B - x_A) \\
    0
  \end{pmatrix} 
.\] 

\[
  \implies \omega = \frac{v_{By} - v_{Ay}}{x_B - x_A}
.\] 

\[
  \cancelto{0}{\vec{v}_C} = \vec{v}_A + \vec{\omega} \times \vec{AC}
.\] 

\[
-\vec{v}_A = \begin{pmatrix} 
  -\omega \cdot (y_C - y_A) \\
  \omega \cdot (x_C - x_A) \\
  0
\end{pmatrix} 
.\] 

\[
\implies
\begin{cases}
  x_C = x_A - \frac{v_{Ay}}{\omega} \\
  y_C = y_A + \frac{v_{Ax}}{\omega}
\end{cases}
.\] 

  \item Ищем центр ускорений по формуле Ривальса.

\[
  \vec{w}_C = 0 = \vec{w}_A + \vec{\varepsilon} \times \vec{AC} - \omega^2 \vec{AC}
.\] 

\[
\begin{pmatrix} 0 \\ 0 \\ \varepsilon \end{pmatrix} =
\begin{pmatrix} 0 \\ 0 \\ \dot \omega \end{pmatrix} 
.\] 

\[
-\vec{w}_A = \begin{pmatrix} 
  -\varepsilon(y_C - y_A) - \omega^2 (x_C - x_A) \\
  \varepsilon (x_C - x_A) - \omega^2 (y_C - y_A) \\
  0
\end{pmatrix} 
.\] 

\[
\implies
\begin{cases}
  \omega^2 (x_C - x_A) = w_{Ax} - \varepsilon(y_C - y_A) \\
  \omega^2 (y_C - y_A) = w_{Ay} + \varepsilon(x_C - x_A)
\end{cases}
.\] 

\[
  \omega^2 (x_C - x_A) = w_{Ax} - \frac{\varepsilon}{\omega^2}
  (w_{Ay} + \varepsilon(x_C - x_A))
.\] 

\[
  (x_C - x_A)\left( \omega^4 + \varepsilon^2 \right) =
  \omega^2 w_{Ax} - \varepsilon w_{Ay}
.\] 

\[
  \boxed{ x_C = x_A + \frac{\omega^2 w_{Ax} - \varepsilon w_{Ay}}
  {\omega^4 + \varepsilon^2}}
.\] 

\[
  \omega^4 (y_C - y_A) = \omega^2 w_{Ay} + \varepsilon
  (w_{Ax} - \varepsilon (y_C - y_A))
.\] 

\[
  (y_C - y_A) \left( \omega^4 + \varepsilon^2 \right)  = \omega^2 w_{Ay} + \varepsilon w_{Ax}
.\] 

\[
  \boxed{ y_C = y_A + \frac{w_{Ay} \omega^2 + \varepsilon w_{Ax}}{\omega^4 + \varepsilon^2}}
.\] 

\end{enumerate}
\end{document}
